theories/lang/pagetable_extra.v
@@ -47,29 +47,29 @@ Proof.
 Qed.
 
 Lemma p_upd_own_current_vm σ i (ps: gset PID):
- get_current_vm (update_ownership_global σ i ps) = get_current_vm σ.
+ get_current_vm (update_page_table_global update_ownership σ i ps) = get_current_vm σ.
 Proof. f_equal. Qed.
 
 Lemma p_upd_own_regs σ i (ps: gset PID):
- get_reg_files (update_ownership_global σ i ps) = get_reg_files σ.
+ get_reg_files (update_page_table_global update_ownership σ i ps) = get_reg_files σ.
 Proof. f_equal. Qed.
 
 Lemma p_upd_own_mem σ i (ps: gset PID):
- get_mem (update_ownership_global σ i ps) = get_mem σ.
+ get_mem (update_page_table_global update_ownership σ i ps) = get_mem σ.
 Proof. f_equal. Qed.
 
-Lemma p_upd_own_mb σ i (ps: gset PID):
- get_mail_boxes (update_ownership_global σ i ps) = get_mail_boxes σ.
+Lemma p_upd_pgt_mb σ i (ps: gset PID):
+ get_mail_boxes (update_page_table_global update_ownership σ i ps) = get_mail_boxes σ.
 Proof. f_equal. Qed.
 
 Lemma p_upd_own_trans σ i (ps: gset PID):
- get_transactions (update_ownership_global σ i ps) = get_transactions σ.
+ get_transactions (update_page_table_global update_ownership σ i ps) = get_transactions σ.
 Proof. f_equal. Qed.
 
 Lemma p_upd_own_access σ i ps:
-((get_access_gmap (update_ownership_global σ i ps)):gmap _ _) = ((get_access_gmap σ): gmap _ _).
+((get_access_gmap (update_page_table_global update_ownership σ i ps)):gmap _ _) = ((get_access_gmap σ): gmap _ _).
 Proof.
-  rewrite /get_access_gmap /update_ownership_global  /=.
+  rewrite /get_access_gmap  /=.
   generalize dependent σ.1.1.1.2.
   induction ps as [|p ps] using set_ind_L.
   done.
@@ -82,15 +82,25 @@ Proof.
   destruct (pgt' !! p) eqn:Hlookup.
   { destruct p1.
     rewrite IHps /=.
-    rewrite fmap_insert /=.
-    apply map_eq.
-    intro.
-    destruct (decide (i0=p)).
-    rewrite e.
-    rewrite lookup_insert.
-    rewrite lookup_fmap  Hlookup.
-    destruct o;done.
-    rewrite lookup_insert_ne;[done|eauto].
+    f_equal.
+    apply (list_eq_same_length _ _ vm_count).
+    rewrite fmap_length.
+    apply length_list_of_vmids.
+    rewrite fmap_length.
+    apply length_list_of_vmids.
+    intros ? ? ? ? H0 H1.
+    apply list_lookup_fmap_inv in H0, H1.
+    destruct H0, H1.
+    destruct H0, H1.
+    rewrite H3 in H4.
+    inversion H4. subst x1.
+    clear H4.
+    rewrite H0 H1.
+    do 4 f_equal.
+    destruct p1.
+    destruct o;
+    rewrite fmap_insert insert_id //.
+    all: rewrite /= lookup_fmap Hlookup //.
   }
   rewrite IHps //.
   }
@@ -99,29 +109,29 @@ Proof.
 Qed.
 
 Lemma p_grnt_acc_current_vm σ i (ps: gset PID) :
- get_current_vm (grant_access_global σ i ps) = get_current_vm σ.
+ get_current_vm (update_page_table_global grant_access σ i ps) = get_current_vm σ.
 Proof. f_equal. Qed.
 
 Lemma p_grnt_acc_regs σ i (ps: gset PID):
- get_reg_files (grant_access_global σ i ps) = get_reg_files σ.
+ get_reg_files (update_page_table_global grant_access σ i ps) = get_reg_files σ.
 Proof. f_equal. Qed.
 
 Lemma p_grnt_acc_mem σ i (ps: gset PID):
- get_mem (grant_access_global σ i ps) = get_mem σ.
+ get_mem (update_page_table_global grant_access σ i ps) = get_mem σ.
 Proof. f_equal. Qed.
 
 Lemma p_grnt_acc_mb σ i (ps: gset PID):
- get_mail_boxes (grant_access_global σ i ps) = get_mail_boxes σ.
+ get_mail_boxes (update_page_table_global grant_access σ i ps) = get_mail_boxes σ.
 Proof. f_equal. Qed.
 
 Lemma p_grnt_acc_trans σ i (ps: gset PID):
- get_transactions (grant_access_global σ i ps) = get_transactions σ.
+ get_transactions (update_page_table_global grant_access σ i ps) = get_transactions σ.
 Proof. f_equal. Qed.
 
 Lemma p_grnt_acc_ownerships σ i ps:
- (get_owned_gmap (grant_access_global σ i ps)) = (get_owned_gmap σ).
+ (get_own_gmap (update_page_table_global grant_access σ i ps)) = (get_own_gmap σ).
 Proof.
-  rewrite /get_owned_gmap /grant_access_global  /=.
+  rewrite /get_own_gmap /=.
   generalize dependent σ.1.1.1.2.
   induction ps as [|p ps] using set_ind_L.
   done.
@@ -149,29 +159,29 @@ Proof.
   Qed.
 
 Lemma p_rvk_acc_current_vm σ i l:
-  get_current_vm (revoke_access_global σ i l) = get_current_vm σ.
+  get_current_vm (update_page_table_global revoke_access σ i l) = get_current_vm σ.
 Proof. f_equal. Qed.
 
 Lemma p_rvk_acc_regs σ i l:
-  get_reg_files (revoke_access_global σ i l) = get_reg_files σ.
+  get_reg_files (update_page_table_global revoke_access σ i l) = get_reg_files σ.
 Proof. f_equal. Qed.
 
 Lemma p_rvk_acc_mem σ i l:
-  get_mem (revoke_access_global σ i l) = get_mem σ.
+  get_mem (update_page_table_global revoke_access σ i l) = get_mem σ.
 Proof. f_equal. Qed.
 
 Lemma p_rvk_acc_mb σ i l:
-  get_mail_boxes (revoke_access_global σ i l) = get_mail_boxes σ.
+  get_mail_boxes (update_page_table_global revoke_access σ i l) = get_mail_boxes σ.
 Proof. f_equal. Qed.
 
 Lemma p_rvk_acc_trans σ i l:
-  get_transactions (revoke_access_global σ i l) = get_transactions σ.
+  get_transactions (update_page_table_global revoke_access σ i l) = get_transactions σ.
 Proof. f_equal. Qed.
 
 Lemma p_rvk_acc_ownerships σ i ps:
- (get_owned_gmap (revoke_access_global σ i ps)) = (get_owned_gmap σ).
+ (get_own_gmap (update_page_table_global revoke_access σ i ps)) = (get_own_gmap σ).
 Proof.
-  rewrite /get_owned_gmap /revoke_access_global  /=.
+  rewrite /get_own_gmap /=.
   generalize dependent σ.1.1.1.2.
   induction ps as [|p ps] using set_ind_L.
   done.
@@ -200,39 +210,40 @@ Qed.
 
 (*--- prove having mappings in gmap implies owership/access to pages in opsem ---*)
 
-Lemma u_rvk_acc_acc σ ps v :
-  get_access_gmap (revoke_access_global σ v ps) = revoke_acc_gmap (get_access_gmap σ) v ps.
-Proof.
-  rewrite /get_access_gmap.
-  rewrite /revoke_access_global /update_page_table_global /=.
-  rewrite /revoke_acc_gmap /update_acc_gmap /=.
-  generalize  σ.1.1.1.2.
-  induction ps as [|p ps] using set_ind_L.
-  intros.
-  rewrite !set_fold_empty //.
-  intro pgt.
-  rewrite !set_fold_disj_union_strong /=.
-  rewrite !set_fold_singleton.
-  rewrite IHps.
-  rewrite lookup_fmap.
-  destruct (pgt!! p) eqn:Hlookup.
-  { rewrite Hlookup /=.
-    destruct p0.
-    simpl.
-    f_equal.
-    rewrite fmap_insert //=.
-  }
-  { rewrite Hlookup //=. }
-  2,4 : set_solver + H.
-  {
-    intros.
-    destruct (b' !! x2) as [p2|] eqn: Hlookup2, (b' !! x1) as [p1|] eqn:Hlookup1;
-      try destruct p1 as [q1 []]; try destruct p2 as [q2 []]; rewrite ?lookup_insert_ne ?Hlookup1 ?Hlookup2 //;last eauto.
-    apply insert_commute.
-    done.
-  }
-  apply upd_is_strong_assoc_comm.
-Qed.
+(* TODO *)
+(* Lemma u_rvk_acc_acc σ ps v : *)
+(*   get_access_gmap (revoke_access_global σ v ps) = revoke_acc_gmap (get_access_gmap σ) v ps. *)
+(* Proof. *)
+(*   rewrite /get_access_gmap. *)
+(*   rewrite /revoke_access_global /update_page_table_global /=. *)
+(*   rewrite /revoke_acc_gmap /update_acc_gmap /=. *)
+(*   generalize  σ.1.1.1.2. *)
+(*   induction ps as [|p ps] using set_ind_L. *)
+(*   intros. *)
+(*   rewrite !set_fold_empty //. *)
+(*   intro pgt. *)
+(*   rewrite !set_fold_disj_union_strong /=. *)
+(*   rewrite !set_fold_singleton. *)
+(*   rewrite IHps. *)
+(*   rewrite lookup_fmap. *)
+(*   destruct (pgt!! p) eqn:Hlookup. *)
+(*   { rewrite Hlookup /=. *)
+(*     destruct p0. *)
+(*     simpl. *)
+(*     f_equal. *)
+(*     rewrite fmap_insert //=. *)
+(*   } *)
+(*   { rewrite Hlookup //=. } *)
+(*   2,4 : set_solver + H. *)
+(*   { *)
+(*     intros. *)
+(*     destruct (b' !! x2) as [p2|] eqn: Hlookup2, (b' !! x1) as [p1|] eqn:Hlookup1; *)
+(*       try destruct p1 as [q1 []]; try destruct p2 as [q2 []]; rewrite ?lookup_insert_ne ?Hlookup1 ?Hlookup2 //;last eauto. *)
+(*     apply insert_commute. *)
+(*     done. *)
+(*   } *)
+(*   apply upd_is_strong_assoc_comm. *)
+(* Qed. *)
 
 Lemma update_page_table_lookup_not_elem_of {i:VMID} {perm : permission} pgt upd (sps: gset PID) (p:PID) :
   p ∉ sps ->
